src/proofs/no_slashable_attestations/supporting_lemmas/dv_next_preserves_ind_inv/invs_dv_next_2.dfy
@@ -563,7 +563,7 @@ module Invs_DV_Next_2
                         assert inv_exists_honest_dvc_that_sent_att_share_for_submitted_att(s');
                 }
 
-            case AdeversaryTakingStep(node, new_attestation_share_sent, messagesReceivedByTheNode) =>
+            case AdeversaryTakingStep(node, new_attestation_shares_sent, messagesReceivedByTheNode) =>
                 forall a | 
                     && a in s'.all_attestations_created
                     && is_valid_attestation(a, s'.dv_pubkey)
@@ -703,7 +703,7 @@ module Invs_DV_Next_2
 
                 }
 
-            case AdeversaryTakingStep(node, new_attestation_share_sent, messagesReceivedByTheNode) =>
+            case AdeversaryTakingStep(node, new_attestation_shares_sent, messagesReceivedByTheNode) =>
 
         }
     }     
@@ -1065,7 +1065,7 @@ module Invs_DV_Next_2
                 assert inv_decided_value_of_consensus_instance_is_decided_by_quorum(s');
                
 
-            case AdeversaryTakingStep(node, new_attestation_share_sent, messagesReceivedByTheNode) =>
+            case AdeversaryTakingStep(node, new_attestation_shares_sent, messagesReceivedByTheNode) =>
                 assert inv_decided_value_of_consensus_instance_is_decided_by_quorum(s');
         }        
     } 
@@ -1238,7 +1238,7 @@ module Invs_DV_Next_2
                 }
                 assert inv_sent_validity_predicate_is_based_on_rcvd_att_duty_and_slashing_db(s');
 
-            case AdeversaryTakingStep(node, new_attestation_share_sent, messagesReceivedByTheNode) =>
+            case AdeversaryTakingStep(node, new_attestation_shares_sent, messagesReceivedByTheNode) =>
                 assert inv_sent_validity_predicate_is_based_on_rcvd_att_duty_and_slashing_db(s');
         }
     }   
@@ -1769,7 +1769,7 @@ module Invs_DV_Next_2
     requires inv_sent_validity_predicate_is_based_on_rcvd_att_duty_and_slashing_db_for_dvc_single_dvc_2(process) 
     ensures inv_sent_validity_predicate_is_based_on_rcvd_att_duty_and_slashing_db_for_dvc_single_dvc_2(s'); 
     {
-        if pred_att_duty_was_already_decided(process, id) 
+        if  is_decided_data_for_current_slot(process, decided_attestation_data, id)
         {
             var s_mod := f_update_process_after_att_duty_decided(
                             process,
@@ -1894,7 +1894,7 @@ module Invs_DV_Next_2
                 }            
 
 
-            case AdeversaryTakingStep(node, new_attestation_share_sent, messagesReceivedByTheNode) =>
+            case AdeversaryTakingStep(node, new_attestation_shares_sent, messagesReceivedByTheNode) =>
                 assert inv_sent_validity_predicate_is_based_on_rcvd_att_duty_and_slashing_db_for_dv(s');
         }        
     } 
@@ -1966,7 +1966,7 @@ module Invs_DV_Next_2
             case HonestNodeTakingStep(node, nodeEvent, nodeOutputs) =>
                 assert s'.sequence_attestation_duties_to_be_served == s.sequence_attestation_duties_to_be_served;
             
-            case AdeversaryTakingStep(node, new_attestation_share_sent, messagesReceivedByTheNode) =>
+            case AdeversaryTakingStep(node, new_attestation_shares_sent, messagesReceivedByTheNode) =>
                 assert s'.sequence_attestation_duties_to_be_served == s.sequence_attestation_duties_to_be_served;
         }
         assert s'.sequence_attestation_duties_to_be_served == s.sequence_attestation_duties_to_be_served;
@@ -2145,7 +2145,7 @@ module Invs_DV_Next_2
     //             }
 
 
-    //         case AdeversaryTakingStep(node, new_attestation_share_sent, messagesReceivedByTheNode) =>
+    //         case AdeversaryTakingStep(node, new_attestation_shares_sent, messagesReceivedByTheNode) =>
     //         //     lem_inv_data_of_att_share_is_decided_value_att_adversary(s, event, s');
     //     }        
     // }
@@ -2232,7 +2232,7 @@ module Invs_DV_Next_2
                     lem_inv_data_of_att_share_is_decided_value_helper(s, event, s');
                 }
 
-            case AdeversaryTakingStep(node, new_attestation_share_sent, messagesReceivedByTheNode) =>
+            case AdeversaryTakingStep(node, new_attestation_shares_sent, messagesReceivedByTheNode) =>
                 lem_inv_data_of_att_share_is_decided_value_att_adversary(s, event, s');
         }        
     }
