src/proofs/no_slashable_attestations/supporting_lemmas/dv_next_preserves_ind_inv/invs_dv_next_5.dfy
@@ -252,7 +252,7 @@ module Invs_DV_Next_5
                 }  
 
                          
-            case AdeversaryTakingStep(node, new_attestation_share_sent, messagesReceivedByTheNode) => 
+            case AdeversaryTakingStep(node, new_attestation_shares_sent, messagesReceivedByTheNode) => 
                 assert s'.consensus_on_attestation_data == s.consensus_on_attestation_data;
                 assert s.honest_nodes_states[hn] == s'.honest_nodes_states[hn];
                  
@@ -637,7 +637,7 @@ module Invs_DV_Next_5
                 }  
 
                          
-            case AdeversaryTakingStep(node, new_attestation_share_sent, messagesReceivedByTheNode) => 
+            case AdeversaryTakingStep(node, new_attestation_shares_sent, messagesReceivedByTheNode) => 
                 assert s'.consensus_on_attestation_data == s.consensus_on_attestation_data;
                 assert s.honest_nodes_states[hn] == s'.honest_nodes_states[hn];
                  
@@ -1047,7 +1047,7 @@ module Invs_DV_Next_5
                 }  
                 assert inv_exists_att_duty_in_dv_seq_of_att_duty_for_every_slot_in_att_slashing_db_hist(s');
                          
-            case AdeversaryTakingStep(node, new_attestation_share_sent, messagesReceivedByTheNode) =>
+            case AdeversaryTakingStep(node, new_attestation_shares_sent, messagesReceivedByTheNode) =>
                 forall hn |
                     && hn in s'.honest_nodes_states.Keys   
                 ensures inv_exists_att_duty_in_dv_seq_of_att_duty_for_every_slot_in_att_slashing_db_hist_body(s', hn, s'.honest_nodes_states[hn], s'.index_next_attestation_duty_to_be_served); 
@@ -1220,6 +1220,30 @@ module Invs_DV_Next_5
         
     }    
 
+    lemma lem_inv_slot_of_consensus_instance_is_up_to_slot_of_latest_attestation_duty(
+        s: DVState,
+        event: DV.Event,
+        s': DVState
+    )
+    requires inv_exists_att_duty_in_dv_seq_of_att_duty_for_every_slot_in_att_slashing_db_hist_a(s)
+    requires inv_active_attestation_consensus_instances_keys_is_subset_of_att_slashing_db_hist(s)   
+    requires inv_latest_attestation_duty_is_from_dv_seq_of_att_duties(s)
+    requires is_sequence_attestation_duties_to_be_served_orderd(s)
+    requires inv_slot_of_consensus_instance_is_up_to_slot_of_latest_attestation_duty(s)
+    requires NextEventPreCond(s, event)
+    requires NextEvent(s, event, s')  
+    ensures inv_slot_of_consensus_instance_is_up_to_slot_of_latest_attestation_duty(s')
+    {
+        match event 
+        {
+            case HonestNodeTakingStep(node, nodeEvent, nodeOutputs) =>
+                lem_inv_slot_of_consensus_instance_is_up_to_slot_of_latest_served_att_duty(s, event, s');
+                
+            case AdeversaryTakingStep(node, new_attestation_shares_sent, messagesReceivedByTheNode) =>
+                
+        }
+    }
+
     lemma lem_inv_slot_of_consensus_instance_is_up_to_slot_of_latest_served_att_duty(
         s: DVState,
         event: DV.Event,
@@ -1340,7 +1364,7 @@ module Invs_DV_Next_5
                 }  
                 assert inv_exists_att_duty_in_dv_seq_of_att_duty_for_every_slot_in_att_slashing_db_hist_a(s');
                          
-            case AdeversaryTakingStep(node, new_attestation_share_sent, messagesReceivedByTheNode) =>
+            case AdeversaryTakingStep(node, new_attestation_shares_sent, messagesReceivedByTheNode) =>
 
         }
     }   
@@ -1509,7 +1533,7 @@ module Invs_DV_Next_5
                     dv'
                 );    
 
-            case AdeversaryTakingStep(node, new_attestation_share_sent, messagesReceivedByTheNode) =>
+            case AdeversaryTakingStep(node, new_attestation_shares_sent, messagesReceivedByTheNode) =>
                 assert inv_decided_data_has_an_honest_witness(dv');
         }   
     }          
@@ -1585,11 +1609,11 @@ module Invs_DV_Next_5
                 assert inv_outputs_attestations_submited_are_valid(nodeOutputs, dv.dv_pubkey);
                 assert inv_all_created_attestations_are_valid(dv');
 
-            case AdeversaryTakingStep(node, new_attestation_share_sent, messagesReceivedByTheNode) =>
+            case AdeversaryTakingStep(node, new_attestation_shares_sent, messagesReceivedByTheNode) =>
                 assert NextAdversary(
                     dv,
                     node,
-                    new_attestation_share_sent,
+                    new_attestation_shares_sent,
                     messagesReceivedByTheNode,
                     dv'
                 );
@@ -1604,7 +1628,659 @@ module Invs_DV_Next_5
                                 
                 assert inv_all_created_attestations_are_valid(dv');
         }  
-    }         
+    }        
+
+    lemma lem_pred_unchanged_rs_dv_next(
+        dv: DVState,
+        event: DV.Event,
+        dv': DVState
+    )    
+    requires NextEventPreCond(dv, event)
+    requires NextEvent(dv, event, dv')  
+    ensures ( forall hn: BLSPubkey | is_honest_node(dv, hn) ::
+                    dv.honest_nodes_states[hn].rs.pubkey
+                    ==
+                    dv'.honest_nodes_states[hn].rs.pubkey
+            )
+    {
+
+    }
+
+    lemma lem_unique_owner_of_att_share(
+        rs_pubkey: BLSPubkey,
+        rs_pubkey': BLSPubkey,
+        att_share: AttestationShare
+    )
+    requires pred_verify_owner_of_attestation_share_with_bls_signature(rs_pubkey, att_share)
+    requires pred_verify_owner_of_attestation_share_with_bls_signature(rs_pubkey', att_share)
+    ensures rs_pubkey == rs_pubkey'
+    {
+        var decided_attestation_data := att_share.data;
+        var fork_version := bn_get_fork_version(compute_start_slot_at_epoch(decided_attestation_data.target.epoch));
+        var attestation_signing_root := compute_attestation_signing_root(decided_attestation_data, fork_version);
+        assert verify_bls_signature(attestation_signing_root, att_share.signature, rs_pubkey);
+        assert verify_bls_signature(attestation_signing_root, att_share.signature, rs_pubkey');
+        rs_attestation_sign_and_verification_propeties();
+        assert rs_pubkey == rs_pubkey';
+    }
+
+    lemma lem_inv_unchanged_dvc_rs_pubkey_dv_next(
+        dv: DVState,
+        event: DV.Event,
+        dv': DVState
+    )    
+    requires NextEventPreCond(dv, event)
+    requires NextEvent(dv, event, dv')  
+    requires inv_unchanged_dvc_rs_pubkey(dv)
+    ensures inv_unchanged_dvc_rs_pubkey(dv')
+    {
+
+    }
+
+    lemma lem_different_signers_cannot_generate_the_same_att_share(
+        rs_pubkey: BLSPubkey,
+        rs_pubkey': BLSPubkey,
+        att_share: AttestationShare
+    )
+    requires rs_pubkey != rs_pubkey'
+    requires pred_verify_owner_of_attestation_share_with_bls_signature(rs_pubkey, att_share)
+    ensures !pred_verify_owner_of_attestation_share_with_bls_signature(rs_pubkey', att_share)
+    {
+        if pred_verify_owner_of_attestation_share_with_bls_signature(rs_pubkey', att_share)
+        {
+            lem_unique_owner_of_att_share(rs_pubkey, rs_pubkey', att_share);
+        }        
+    }
+
+    lemma lem_inv_honest_nodes_are_not_owner_of_att_shares_from_adversary(
+        dv: DVState
+    )
+    requires inv_quorum_constraints(dv)
+    ensures inv_honest_nodes_are_not_owner_of_att_shares_from_adversary(dv)
+    {
+        var honest_nodes := dv.honest_nodes_states.Keys;
+        var dishonest_nodes := dv.adversary.nodes;
+        lemmaEmptyIntersectionImpliesDisjointness(honest_nodes, dishonest_nodes);
+        assert honest_nodes !! dishonest_nodes;
+
+        forall byz_node: BLSPubkey, att_share: AttestationShare | 
+            && byz_node in dv.adversary.nodes 
+            && att_share in dv.att_network.allMessagesSent
+            && pred_verify_owner_of_attestation_share_with_bls_signature(byz_node, att_share)
+        ensures inv_honest_nodes_are_not_owner_of_att_shares_from_adversary_body(dv, att_share)
+        {
+            forall hn: BLSPubkey | is_honest_node(dv, hn)
+            ensures !pred_verify_owner_of_attestation_share_with_bls_signature(hn, att_share)
+            {
+                assert hn != byz_node;
+                lem_different_signers_cannot_generate_the_same_att_share(
+                    byz_node,
+                    hn,
+                    att_share
+                );
+                assert !pred_verify_owner_of_attestation_share_with_bls_signature(hn, att_share);
+            }
+        }
+    }
+
+    // 2 minutes
+    lemma lem_inv_data_of_att_shares_is_known_dv_next(
+        dv: DVState,
+        event: DV.Event,
+        dv': DVState
+    )    
+    requires NextEventPreCond(dv, event)
+    requires NextEvent(dv, event, dv')  
+    requires inv_quorum_constraints(dv)
+    requires inv_data_of_att_shares_is_known(dv)
+    requires inv_unchanged_dvc_rs_pubkey(dv)
+    requires inv_att_shares_to_broadcast_is_tracked_in_attestation_slashing_db(dv)
+    ensures  inv_data_of_att_shares_is_known(dv')
+    {        
+        match event 
+        {
+            case HonestNodeTakingStep(node, nodeEvent, nodeOutputs) =>
+                var dvc := dv.honest_nodes_states[node];
+                var dvc' := dv'.honest_nodes_states[node];
+                match nodeEvent
+                {
+                    case ServeAttstationDuty(attestation_duty) =>     
+                        lem_inv_outputs_attestation_shares_sent_is_tracked_in_attestation_slashing_db_f_serve_attestation_duty(dvc, attestation_duty, dvc');
+                        assert inv_outputs_attestation_shares_sent_is_tracked_in_attestation_slashing_db(nodeOutputs, dvc');  
+                        
+                    case AttConsensusDecided(id, decided_attestation_data) => 
+                        if f_att_consensus_decided.requires(dvc, id, decided_attestation_data)
+                        {
+                            lem_inv_outputs_attestation_shares_sent_is_tracked_in_attestation_slashing_db_f_att_consensus_decided(dvc, id, decided_attestation_data, dvc');      
+                            assert inv_outputs_attestation_shares_sent_is_tracked_in_attestation_slashing_db(nodeOutputs, dvc');  
+                        }                 
+                        
+                    case ReceivedAttestationShare(attestation_share) =>                         
+                        lem_inv_outputs_attestation_shares_sent_is_tracked_in_attestation_slashing_db_f_listen_for_attestation_shares(dvc, attestation_share, dvc');                        
+                        assert inv_outputs_attestation_shares_sent_is_tracked_in_attestation_slashing_db(nodeOutputs, dvc');  
+   
+                    case ImportedNewBlock(block) => 
+                        var dvc := f_add_block_to_bn(dvc, nodeEvent.block);
+                        lem_inv_outputs_attestation_shares_sent_is_tracked_in_attestation_slashing_db_f_listen_for_new_imported_blocks(dvc, block, dvc');
+                        assert inv_outputs_attestation_shares_sent_is_tracked_in_attestation_slashing_db(nodeOutputs, dvc');  
+                                                
+                    case ResendAttestationShares =>       
+                        lem_inv_outputs_attestation_shares_sent_is_tracked_in_attestation_slashing_db_f_resend_attestation_share(dvc, dvc');
+                        assert inv_outputs_attestation_shares_sent_is_tracked_in_attestation_slashing_db(nodeOutputs, dvc');                    
+                        
+                    case NoEvent => 
+                        assert inv_outputs_attestation_shares_sent_is_tracked_in_attestation_slashing_db(nodeOutputs, dvc');  
+                }
+                
+                assert inv_outputs_attestation_shares_sent_is_tracked_in_attestation_slashing_db(nodeOutputs, dvc');
+
+                assert  dv.att_network.allMessagesSent + getMessagesFromMessagesWithRecipient(nodeOutputs.att_shares_sent)
+                        ==
+                        dv'.att_network.allMessagesSent
+                        ;
+                forall hn: BLSPubkey, att_share: AttestationShare | 
+                            && is_honest_node(dv, hn)
+                            && att_share in dv'.att_network.allMessagesSent 
+                            && var hn_node': DVCState := dv'.honest_nodes_states[hn];
+                            && var hn_rs_pubkey: BLSPubkey := hn_node'.rs.pubkey;
+                            && pred_verify_owner_of_attestation_share_with_bls_signature(hn_rs_pubkey, att_share)
+                ensures && var hn_node': DVCState := dv'.honest_nodes_states[hn];
+                        && inv_data_of_att_shares_is_known_body(hn_node', att_share)            
+                {
+                    var hn_node: DVCState := dv.honest_nodes_states[hn];
+                    var hn_node': DVCState := dv'.honest_nodes_states[hn];
+                    var hn_rs_pubkey: BLSPubkey := hn_node'.rs.pubkey;
+
+                    lem_pred_unchanged_rs_dv_next(dv, event, dv');         
+                    assert hn_node.rs.pubkey == hn_node'.rs.pubkey;                    
+                    
+
+                    if att_share in dv.att_network.allMessagesSent 
+                    {
+                        assert inv_data_of_att_shares_is_known_body(hn_node, att_share);
+                        assert inv_data_of_att_shares_is_known_body(hn_node', att_share);
+                    }
+                    else
+                    {                        
+                        assert att_share in getMessagesFromMessagesWithRecipient(nodeOutputs.att_shares_sent);
+                        rs_attestation_sign_and_verification_propeties();
+                        assert inv_outputs_attestation_shares_sent_is_tracked_in_attestation_slashing_db_body(
+                                    dvc', 
+                                    att_share
+                                );
+                        assert inv_data_of_att_shares_is_known_body(dvc', att_share);
+                        assert pred_verify_owner_of_attestation_share_with_bls_signature(dvc'.rs.pubkey, att_share);
+                        assert pred_verify_owner_of_attestation_share_with_bls_signature(hn_rs_pubkey, att_share);
+                        lem_unique_owner_of_att_share(hn_rs_pubkey, dvc'.rs.pubkey, att_share);
+                        assert hn_rs_pubkey == dvc'.rs.pubkey;
+
+                        calc 
+                        {
+                            hn;
+                            ==      
+                            { lem_inv_unchanged_dvc_rs_pubkey_dv_next(dv, event, dv'); }
+                            hn_rs_pubkey;
+                            ==
+                            dvc'.rs.pubkey;
+                            ==
+                            { lem_inv_unchanged_dvc_rs_pubkey_dv_next(dv, event, dv'); }
+                            node;
+                        }
+
+                        assert hn_node' == dvc';
+                        assert inv_data_of_att_shares_is_known_body(hn_node', att_share);
+                    }
+                }
+                assert inv_data_of_att_shares_is_known(dv');
+
+            case AdeversaryTakingStep(node, new_attestation_shares_sent, messagesReceivedByTheNode) =>
+                lem_inv_quorum_constraints_dv_next(dv, event, dv');
+                assert inv_quorum_constraints(dv');
+                var dishonest_nodes := dv'.adversary.nodes;
+                var honest_nodes := dv'.honest_nodes_states.Keys;
+                lemmaEmptyIntersectionImpliesDisjointness(dishonest_nodes, honest_nodes);
+                assert dishonest_nodes !! honest_nodes;
+
+                var new_att_shares := dv'.att_network.allMessagesSent - dv.att_network.allMessagesSent;
+                forall new_att_share: AttestationShare, signer: BLSPubkey | 
+                            (   && new_att_share in new_att_shares
+                                && var fork_version := bn_get_fork_version(compute_start_slot_at_epoch(new_att_share.data.target.epoch));
+                                && var attestation_signing_root := compute_attestation_signing_root(new_att_share.data, fork_version);
+                                && verify_bls_signature(attestation_signing_root, new_att_share.signature, signer)
+                            )
+                ensures !is_honest_node(dv, signer)
+                {
+                    assert signer in dishonest_nodes;
+                    assert !is_honest_node(dv, signer);
+                }
+                assert inv_data_of_att_shares_is_known(dv');
+        }  
+    }  
+
+    lemma lem_inv_att_shares_to_broadcast_is_tracked_in_attestation_slashing_db_dv_next(
+        dv: DVState,
+        event: DV.Event,
+        dv': DVState
+    )    
+    requires NextEventPreCond(dv, event)
+    requires NextEvent(dv, event, dv')  
+    requires inv_att_shares_to_broadcast_is_tracked_in_attestation_slashing_db(dv)
+    ensures  inv_att_shares_to_broadcast_is_tracked_in_attestation_slashing_db(dv')
+    {        
+        match event 
+        {
+            case HonestNodeTakingStep(node, nodeEvent, nodeOutputs) =>
+                var dvc := dv.honest_nodes_states[node];
+                var dvc' := dv'.honest_nodes_states[node];
+                match nodeEvent
+                {
+                    case ServeAttstationDuty(attestation_duty) =>     
+                        lem_inv_att_shares_to_broadcast_is_tracked_in_attestation_slashing_db_body_f_serve_attestation_duty(dvc, attestation_duty, dvc');
+                        
+                    case AttConsensusDecided(id, decided_attestation_data) => 
+                        if f_att_consensus_decided.requires(dvc, id, decided_attestation_data)
+                        {
+                            lem_inv_att_shares_to_broadcast_is_tracked_in_attestation_slashing_db_body_f_att_consensus_decided(dvc, id, decided_attestation_data, dvc');      
+                        }                 
+                        
+                    case ReceivedAttestationShare(attestation_share) =>                         
+                        lem_inv_att_shares_to_broadcast_is_tracked_in_attestation_slashing_db_body_f_listen_for_attestation_shares(dvc, attestation_share, dvc');         
+   
+                    case ImportedNewBlock(block) => 
+                        var dvc := f_add_block_to_bn(dvc, nodeEvent.block);
+                        lem_inv_att_shares_to_broadcast_is_tracked_in_attestation_slashing_db_body_f_listen_for_new_imported_blocks(dvc, block, dvc');                        
+                                                
+                    case ResendAttestationShares =>       
+                        
+                    case NoEvent => 
+                }
+                
+            case AdeversaryTakingStep(node, new_attestation_shares_sent, messagesReceivedByTheNode) =>
+                
+        }  
+    }  
+
+    lemma lem_AdeversaryTakingStep_new_att_share_sent_is_not_from_honest_node(
+        dv: DVState,        
+        event: DV.Event,
+        node: BLSPubkey,
+        new_attestation_shares_sent: set<MessaageWithRecipient<AttestationShare>>,
+        messagesReceivedByTheNode: set<AttestationShare>,
+        dv': DVState,
+        pubkey: BLSPubkey,
+        new_att_share_sent: MessaageWithRecipient<AttestationShare>
+    )
+    requires NextEventPreCond(dv, event)
+    requires NextEvent(dv, event, dv') 
+    requires event.AdeversaryTakingStep? 
+    requires NextAdversary(dv, node, new_attestation_shares_sent, messagesReceivedByTheNode, dv')
+    requires inv_quorum_constraints(dv)
+    requires && new_att_share_sent in new_attestation_shares_sent
+             && pred_verify_owner_of_attestation_share_with_bls_signature(pubkey, new_att_share_sent.message)
+    ensures !is_honest_node(dv', pubkey)
+    {
+        
+        var message := new_att_share_sent.message;
+        var att_data := message.data;
+
+        lem_inv_quorum_constraints_dv_next(dv, event, dv');
+        assert inv_quorum_constraints(dv');
+        var dishonest_nodes := dv'.adversary.nodes;
+        var honest_nodes := dv'.honest_nodes_states.Keys;
+        lemmaEmptyIntersectionImpliesDisjointness(dishonest_nodes, honest_nodes);
+        assert dishonest_nodes !! honest_nodes;
+
+        var fork_version := bn_get_fork_version(compute_start_slot_at_epoch(att_data.target.epoch));
+        var attestation_signing_root := compute_attestation_signing_root(att_data, fork_version);
+        assert verify_bls_signature(attestation_signing_root, message.signature, pubkey);
+
+        assert pubkey in dishonest_nodes;
+        assert !is_honest_node(dv, pubkey);
+    }
+
+    lemma lem_AdeversaryTakingStep_att_share_from_honest_node_were_sent_before(
+        dv: DVState,        
+        event: DV.Event,
+        node: BLSPubkey,
+        new_attestation_shares_sent: set<MessaageWithRecipient<AttestationShare>>,
+        messagesReceivedByTheNode: set<AttestationShare>,
+        dv': DVState,
+        pubkey: BLSPubkey,
+        old_att_share: AttestationShare
+    )
+    requires NextEventPreCond(dv, event)
+    requires NextEvent(dv, event, dv') 
+    requires event.AdeversaryTakingStep? 
+    requires NextAdversary(dv, node, new_attestation_shares_sent, messagesReceivedByTheNode, dv')
+    requires inv_quorum_constraints(dv)
+    requires is_honest_node(dv', pubkey)
+    requires && old_att_share in dv'.att_network.allMessagesSent
+             && pred_verify_owner_of_attestation_share_with_bls_signature(pubkey, old_att_share)
+    ensures old_att_share in dv.att_network.allMessagesSent
+    {
+        var att_data := old_att_share.data;
+        var fork_version := bn_get_fork_version(compute_start_slot_at_epoch(att_data.target.epoch));
+        var attestation_signing_root := compute_attestation_signing_root(att_data, fork_version);
+        
+        assert  dv'.att_network.allMessagesSent
+                == 
+                dv.att_network.allMessagesSent + getMessagesFromMessagesWithRecipient(new_attestation_shares_sent);
+
+
+        assert  || old_att_share in dv.att_network.allMessagesSent
+                || old_att_share in getMessagesFromMessagesWithRecipient(new_attestation_shares_sent)
+                ;
+
+        if old_att_share in getMessagesFromMessagesWithRecipient(new_attestation_shares_sent)
+        {
+            if new_attestation_shares_sent == {}
+            {
+                assert {} == getMessagesFromMessagesWithRecipient(new_attestation_shares_sent);
+            }
+            assert {} != getMessagesFromMessagesWithRecipient(new_attestation_shares_sent);
+            var old_att_share_sent :|
+                    && old_att_share_sent in new_attestation_shares_sent
+                    && old_att_share_sent.message == old_att_share
+                    ;
+            var signer: BLSPubkey :| verify_bls_signature(attestation_signing_root, old_att_share.signature, signer);
+            assert signer in dv'.adversary.nodes;     
+            lem_inv_honest_nodes_are_not_owner_of_att_shares_from_adversary(dv');
+            lem_different_signers_cannot_generate_the_same_att_share(
+                signer,
+                pubkey,
+                old_att_share
+            );
+        }
+        assert old_att_share !in getMessagesFromMessagesWithRecipient(new_attestation_shares_sent);
+        assert old_att_share in dv.att_network.allMessagesSent;
+    }
+
+    lemma lem_inv_db_of_vp_contains_all_att_data_of_sent_att_shares_for_lower_slots_dv_next(
+        dv: DVState,
+        event: DV.Event,
+        dv': DVState
+    )    
+    requires NextEventPreCond(dv, event)
+    requires NextEvent(dv, event, dv')  
+    requires inv_unchanged_dvc_rs_pubkey(dv)
+    requires inv_quorum_constraints(dv)
+    requires inv_attestation_shares_to_broadcast_is_a_subset_of_all_messages_sent(dv)
+    requires inv_data_of_att_shares_is_known(dv)
+    requires inv_db_of_vp_contains_all_att_data_of_sent_att_shares_for_lower_slots(dv)
+    requires inv_slot_of_consensus_instance_is_up_to_slot_of_latest_attestation_duty(dv)
+    requires inv_available_current_att_duty_is_latest_served_att_duty(dv)
+    requires inv_exists_att_duty_in_dv_seq_of_att_duty_for_every_slot_in_att_slashing_db_hist_a(dv)
+    requires inv_active_attestation_consensus_instances_keys_is_subset_of_att_slashing_db_hist(dv)   
+    requires inv_latest_attestation_duty_is_from_dv_seq_of_att_duties(dv)
+    requires is_sequence_attestation_duties_to_be_served_orderd(dv)
+    ensures  inv_db_of_vp_contains_all_att_data_of_sent_att_shares_for_lower_slots(dv')
+    {        
+        
+        match event 
+        {
+            case HonestNodeTakingStep(node, nodeEvent, nodeOutputs) =>
+                var dvc := dv.honest_nodes_states[node];
+                var dvc' := dv'.honest_nodes_states[node];
+                match nodeEvent
+                {
+                    case ServeAttstationDuty(attestation_duty) =>  
+                        lem_inv_db_of_vp_contains_all_att_data_of_sent_att_shares_for_lower_slots_dvc_f_serve_attestation_duty(
+                            dv.att_network.allMessagesSent,
+                            dvc,
+                            attestation_duty,
+                            dvc'
+                        );
+                        assert inv_db_of_vp_contains_all_att_data_of_sent_att_shares_for_lower_slots(dv');
+                        
+                    case AttConsensusDecided(id, decided_attestation_data) => 
+                        if f_att_consensus_decided.requires(dvc, id, decided_attestation_data)
+                        {
+                            if  && dvc.current_attestation_duty.isPresent()
+                                && id == dvc.current_attestation_duty.safe_get().slot
+                                && id == decided_attestation_data.slot
+                            {
+                                var allMessagesSent := dv.att_network.allMessagesSent;
+                                
+                                lem_inv_slot_of_consensus_instance_is_up_to_slot_of_latest_attestation_duty(
+                                    dv,
+                                    event,
+                                    dv'
+                                );
+
+                                assert ( forall slot  |
+                                                    slot in dvc'.attestation_consensus_engine_state.att_slashing_db_hist
+                                                    ::
+                                                    slot <= dvc'.latest_attestation_duty.safe_get().slot
+                                        );
+                                lem_inv_db_of_vp_contains_all_att_data_of_sent_att_shares_for_lower_slots_dvc_f_att_consensus_decided_new_att_shares_sent(
+                                            allMessagesSent,
+                                            dvc,
+                                            id,
+                                            decided_attestation_data, 
+                                            dvc'
+                                        );
+                                
+                                var allMessagesSent' := dv'.att_network.allMessagesSent;
+                                var outputs := f_att_consensus_decided(dvc, id, decided_attestation_data).outputs;
+                                assert allMessagesSent' == allMessagesSent + getMessagesFromMessagesWithRecipient(outputs.att_shares_sent);
+
+                                var attestation_with_signature_share := f_calc_att_with_sign_share_from_decided_att_data(
+                                                                        dvc,
+                                                                        id,
+                                                                        decided_attestation_data
+                                                                    );       
+                                var messagesToBeSent := f_att_consensus_decided(dvc, id, decided_attestation_data).outputs.att_shares_sent;
+
+                                assert forall m | m in messagesToBeSent :: m.message == attestation_with_signature_share; 
+
+                                lemmaOnGetMessagesFromMessagesWithRecipientWhenAllMessagesAreTheSame(messagesToBeSent, attestation_with_signature_share);    
+                                assert getMessagesFromMessagesWithRecipient(messagesToBeSent) ==  {attestation_with_signature_share};
+                                assert  dv'.att_network.allMessagesSent 
+                                        == 
+                                        dv.att_network.allMessagesSent + { attestation_with_signature_share }
+                                        ; 
+
+                                forall hn: BLSPubkey, slot: Slot, vp: AttestationData -> bool, db: set<SlashingDBAttestation> | 
+                                            && is_honest_node(dv, hn) 
+                                            && var process' := dv.honest_nodes_states[hn];
+                                            && slot in process'.attestation_consensus_engine_state.att_slashing_db_hist.Keys
+                                            && vp in process'.attestation_consensus_engine_state.att_slashing_db_hist[slot]
+                                            && db in process'.attestation_consensus_engine_state.att_slashing_db_hist[slot][vp]
+                                ensures inv_db_of_vp_contains_all_att_data_of_sent_att_shares_for_lower_slots_body(
+                                            dv',
+                                            hn,
+                                            slot,
+                                            vp,
+                                            db)
+                                {
+                                    var process := dv.honest_nodes_states[hn];
+                                    var process' := dv'.honest_nodes_states[hn];                            
+                                    assert hn == process.rs.pubkey == process'.rs.pubkey;
+
+                                    forall att_share: AttestationShare | 
+                                            && att_share in dv'.att_network.allMessagesSent
+                                            && is_honest_node(dv', hn)
+                                            && pred_verify_owner_of_attestation_share_with_bls_signature(hn, att_share)
+                                            && att_share.data.slot < slot
+                                    ensures && var att_data := att_share.data;
+                                            && var slashing_db_attestation := SlashingDBAttestation(
+                                                            source_epoch := att_data.source.epoch,
+                                                            target_epoch := att_data.target.epoch,
+                                                            signing_root := Some(hash_tree_root(att_data)));
+                                            && slashing_db_attestation in db
+                                    {
+                                        assert  || att_share in dv.att_network.allMessagesSent 
+                                                || att_share in { attestation_with_signature_share }
+                                                ;
+                                        if att_share in dv.att_network.allMessagesSent
+                                        {
+                                            var att_data := att_share.data;
+                                            var slashing_db_attestation := SlashingDBAttestation(
+                                                                source_epoch := att_data.source.epoch,
+                                                                target_epoch := att_data.target.epoch,
+                                                                signing_root := Some(hash_tree_root(att_data)));
+
+                                            assert  && att_share in dv.att_network.allMessagesSent
+                                                    && is_honest_node(dv, hn)
+                                                    && pred_verify_owner_of_attestation_share_with_bls_signature(hn, att_share)
+                                                    && att_share.data.slot < slot
+                                                    ;
+                                            assert slashing_db_attestation in db;                        
+                                        }
+                                        else
+                                        {
+                                            assert att_share == attestation_with_signature_share;
+
+                                            var att_data := att_share.data;
+                                            var fork_version := bn_get_fork_version(compute_start_slot_at_epoch(att_data.target.epoch));
+                                            var attestation_signing_root := compute_attestation_signing_root(att_data, fork_version);
+                                            var signer: BLSPubkey :| 
+                                                    verify_bls_signature(attestation_signing_root, att_share.signature, signer);
+
+                                            assert pred_verify_owner_of_attestation_share_with_bls_signature(dvc'.rs.pubkey, attestation_with_signature_share);
+
+                                            lem_unique_owner_of_att_share(
+                                                signer,
+                                                dvc'.rs.pubkey,
+                                                attestation_with_signature_share
+                                            );
+                                            assert signer == dvc'.rs.pubkey;
+                                            if hn == signer
+                                            {
+                                                assert ( forall slot: Slot | slot in dvc'.attestation_consensus_engine_state.att_slashing_db_hist ::
+                                                        attestation_with_signature_share.data.slot >= slot
+                                                );
+                                            }
+                                            else
+                                            {
+                                                lem_different_signers_cannot_generate_the_same_att_share(
+                                                    dvc'.rs.pubkey,
+                                                    hn,
+                                                    attestation_with_signature_share
+                                                );
+
+                                                assert !pred_verify_owner_of_attestation_share_with_bls_signature(hn, attestation_with_signature_share);
+                                            }
+
+                                        }
+                                    }
+                                    
+                                }
+                                        
+                            }
+                            else
+                            {
+                                assert inv_db_of_vp_contains_all_att_data_of_sent_att_shares_for_lower_slots(dv');
+                            }
+
+                        }                 
+                        assert inv_db_of_vp_contains_all_att_data_of_sent_att_shares_for_lower_slots(dv');
+                        
+                    case ReceivedAttestationShare(attestation_share) =>                         
+   
+                    case ImportedNewBlock(block) => 
+                        var dvc := f_add_block_to_bn(dvc, nodeEvent.block);
+                        lem_inv_db_of_vp_contains_all_att_data_of_sent_att_shares_for_lower_slots_dvc_f_listen_for_new_imported_blocks(
+                            dv.att_network.allMessagesSent,
+                            dvc,
+                            block,
+                            dvc'
+                        );
+                        assert inv_db_of_vp_contains_all_att_data_of_sent_att_shares_for_lower_slots(dv');
+                                                
+                    case ResendAttestationShares =>           
+                        lem_inv_db_of_vp_contains_all_att_data_of_sent_att_shares_for_lower_slots_dvc_f_resend_attestation_share(
+                            dv.att_network.allMessagesSent,
+                            dvc,
+                            dvc'
+                        );
+                        assert  dv.att_network.allMessagesSent == dv'.att_network.allMessagesSent;
+                        assert  inv_db_of_vp_contains_all_att_data_of_sent_att_shares_for_lower_slots_dvc(                
+                                    dv'.att_network.allMessagesSent,
+                                    dvc'
+                                );
+                        assert  inv_db_of_vp_contains_all_att_data_of_sent_att_shares_for_lower_slots(dv');
+                        
+                    case NoEvent =>                         
+                        assert  inv_db_of_vp_contains_all_att_data_of_sent_att_shares_for_lower_slots(dv');
+                }
+
+            case AdeversaryTakingStep(node, new_attestation_shares_sent, messagesReceivedByTheNode) =>
+                lem_inv_unchanged_dvc_rs_pubkey_dv_next(dv, event, dv');
+        
+                forall hn: BLSPubkey, slot: Slot, vp: AttestationData -> bool, db: set<SlashingDBAttestation> | 
+                            && is_honest_node(dv, hn) 
+                            && var dvc' := dv.honest_nodes_states[hn];
+                            && slot in dvc'.attestation_consensus_engine_state.att_slashing_db_hist
+                            && vp in dvc'.attestation_consensus_engine_state.att_slashing_db_hist[slot]
+                            && db in dvc'.attestation_consensus_engine_state.att_slashing_db_hist[slot][vp]
+                ensures inv_db_of_vp_contains_all_att_data_of_sent_att_shares_for_lower_slots_body(
+                            dv',
+                            hn,
+                            slot,
+                            vp,
+                            db)
+                {
+                    var dvc := dv.honest_nodes_states[hn];
+                    var dvc' := dv'.honest_nodes_states[hn];
+                    assert dvc == dvc';
+                    assert db in dvc.attestation_consensus_engine_state.att_slashing_db_hist[slot][vp];
+
+                    assert inv_db_of_vp_contains_all_att_data_of_sent_att_shares_for_lower_slots_body(
+                            dv,
+                            hn,
+                            slot, 
+                            vp, 
+                            db
+                        );
+                    
+                    assert hn == dvc.rs.pubkey;
+
+                    forall att_share: AttestationShare | 
+                            && att_share in dv'.att_network.allMessagesSent
+                            && is_honest_node(dv', hn)
+                            && pred_verify_owner_of_attestation_share_with_bls_signature(hn, att_share)
+                            && att_share.data.slot < slot
+                    ensures &&  var att_data := att_share.data;
+                            && var slashing_db_attestation := SlashingDBAttestation(
+                                            source_epoch := att_data.source.epoch,
+                                            target_epoch := att_data.target.epoch,
+                                            signing_root := Some(hash_tree_root(att_data)));
+                            && slashing_db_attestation in db
+                    {
+                        lem_AdeversaryTakingStep_att_share_from_honest_node_were_sent_before(
+                            dv,        
+                            event,
+                            node,
+                            new_attestation_shares_sent,
+                            messagesReceivedByTheNode,
+                            dv',
+                            hn,
+                            att_share
+                        );
+                        assert att_share in dv.att_network.allMessagesSent;
+
+                        var att_data := att_share.data;
+                        var slashing_db_attestation := SlashingDBAttestation(
+                                            source_epoch := att_data.source.epoch,
+                                            target_epoch := att_data.target.epoch,
+                                            signing_root := Some(hash_tree_root(att_data)));
+
+                        assert  && att_share in dv.att_network.allMessagesSent
+                                && is_honest_node(dv, hn)
+                                && pred_verify_owner_of_attestation_share_with_bls_signature(hn, att_share)
+                                && att_share.data.slot < slot
+                                ;
+                        assert slashing_db_attestation in db;                        
+                    }
+                    
+                }
+
+                assert inv_db_of_vp_contains_all_att_data_of_sent_att_shares_for_lower_slots(dv');
+            
+        }  
+    }    
+
 
     lemma lem_inv_attestation_is_created_with_shares_from_quorum_dv_next(
         dv: DVState,
@@ -1617,12 +2293,21 @@ module Invs_DV_Next_5
     requires invNetwork(dv)
     requires inv_rcvd_attestation_shares_is_in_all_messages_sent(dv)
     requires inv_attestation_is_created_with_shares_from_quorum(dv)
+    requires inv_unchanged_dvc_rs_pubkey(dv)
+    requires inv_attestation_is_created_with_shares_from_quorum(dv)
     ensures  inv_attestation_is_created_with_shares_from_quorum(dv')
     {        
         lem_inv_only_dv_construct_signed_attestation_signature_dv_next(dv, event, dv');
         assert inv_only_dv_construct_signed_attestation_signature(dv');
 
+        lem_inv_unchanged_dvc_rs_pubkey_dv_next(dv, event, dv');
+        assert ( forall hn: BLSPubkey | is_honest_node(dv, hn) ::
+                        && hn == dv.honest_nodes_states[hn].rs.pubkey
+                        && hn == dv'.honest_nodes_states[hn].rs.pubkey
+        );
+
         lem_inv_rcvd_attestation_shares_is_in_all_messages_sent(dv, event, dv');
+
 
         match event 
         {
@@ -1661,21 +2346,71 @@ module Invs_DV_Next_5
                 {
                     if att in dv.all_attestations_created 
                     {
+                        assert inv_attestation_is_created_with_shares_from_quorum_body(dv, att);
+                        var att_shares, dvc_signer_pubkeys :|
+                                && att_shares <= dv.att_network.allMessagesSent
+                                && var constructed_sig := dv.construct_signed_attestation_signature(att_shares);
+                                && constructed_sig.isPresent()
+                                && constructed_sig.safe_get() == att.signature
+                                && do_all_att_shares_have_the_same_data(att_shares, att.data)
+                                && dvc_signer_pubkeys <= dv.all_nodes
+                                && inv_attestation_is_created_with_shares_from_quorum_body_signers(dv, att_shares, dvc_signer_pubkeys)
+                                && |dvc_signer_pubkeys| >= quorum(|dv.all_nodes|)
+                                && dvc_signer_pubkeys <= dv.all_nodes
+                                ;
+                        var constructed_sig := dv.construct_signed_attestation_signature(att_shares);
+
+                        assert dv.att_network.allMessagesSent <= dv'.att_network.allMessagesSent;
+                        assert att_shares <= dv'.att_network.allMessagesSent;
+
+                        lem_inv_only_dv_construct_signed_attestation_signature_dv_next(dv, event, dv');                        
+                        assert constructed_sig == dv'.construct_signed_attestation_signature(att_shares);
+                        assert dvc_signer_pubkeys <= dv'.all_nodes;
+                        assert inv_attestation_is_created_with_shares_from_quorum_body_signers(dv', att_shares, dvc_signer_pubkeys);
                         assert inv_attestation_is_created_with_shares_from_quorum_body(dv', att);
                     }
                     else
                     {
                         assert att in nodeOutputs.attestations_submitted;
+                        assert inv_outputs_attestations_submited_is_created_with_shares_from_quorum_body(dvc', att);
+                        var att_shares, rs_signer_pubkeys, k :|        
+                                    && k in dvc'.rcvd_attestation_shares[att.data.slot].Keys
+                                    && att_shares <= dvc'.rcvd_attestation_shares[att.data.slot][k]
+                                    && var constructed_sig := dvc'.construct_signed_attestation_signature(att_shares);
+                                    && constructed_sig.isPresent()
+                                    && constructed_sig.safe_get() == att.signature
+                                    && do_all_att_shares_have_the_same_data(att_shares, att.data)
+                                    && inv_attestation_is_created_with_shares_from_quorum_rs_signers(att_shares, rs_signer_pubkeys)
+                                    && |rs_signer_pubkeys| >= quorum(|dvc'.peers|)
+                                    && rs_signer_pubkeys <= dvc'.peers
+                                    ;
+                        var constructed_sig := dvc'.construct_signed_attestation_signature(att_shares);
+
+                        assert  dvc'.peers == dv'.all_nodes;
+                        assert  quorum(|dvc'.peers|) == quorum(|dv'.all_nodes|);
+                        assert  && |rs_signer_pubkeys| >= quorum(|dvc'.peers|)
+                                && rs_signer_pubkeys <= dv'.all_nodes;
+
+                        
+
+                        lem_inv_only_dv_construct_signed_attestation_signature_dv_next(dv, event, dv');                        
+                        assert constructed_sig == dv'.construct_signed_attestation_signature(att_shares);
+                        assert inv_attestation_is_created_with_shares_from_quorum_body_signers(dv', att_shares, rs_signer_pubkeys);
+
+                        lem_inv_rcvd_attestation_shares_is_in_all_messages_sent(dv, event, dv');  
+                        assert dvc'.rcvd_attestation_shares[att.data.slot][k] <= dv'.att_network.allMessagesSent;   
+                        assert att_shares <= dv'.att_network.allMessagesSent;   
+
                         assert inv_attestation_is_created_with_shares_from_quorum_body(dv', att);
                     }
                 }
                 assert inv_attestation_is_created_with_shares_from_quorum(dv');
 
-            case AdeversaryTakingStep(node, new_attestation_share_sent, messagesReceivedByTheNode) =>
+            case AdeversaryTakingStep(node, new_attestation_shares_sent, messagesReceivedByTheNode) =>
                 assert NextAdversary(
                     dv,
                     node,
-                    new_attestation_share_sent,
+                    new_attestation_shares_sent,
                     messagesReceivedByTheNode,
                     dv'
                 );
